## mess up, find why didn't work

$$\frac{w}{-2} + \frac{1}{6} = \frac{2}{3}$$

* **after moving $\frac{1}{6}$**
    $$\frac{w}{-2} = \frac{2}{3} - \frac{1}{6}$$

* **Denominators:** 3, and 6, **LCM:** 6

* **Simplify based on LCM for RHS:**

    $$\left(\frac{w}{-2}\right) = 6 \cdot \left(\frac{2}{3}\right) - 6 \cdot \left(\frac{1}{6}\right)$$
    * **Simplify**
    $$\left(\frac{w}{-2}\right) = \cancel{6} 2 \cdot \left(\frac{2}{\cancel{3}}\right) - \cancel{6} \cdot \left(\frac{1}{\cancel{6}}\right)$$
    $$\frac{w}{-2} = (2 * 2) - 1$$
    $$\frac{w}{-2} = 3$$

because we are doing clearing denominator in the operation, clearning denominator means we are modifying the equation, it has to be done in both side


we are mixing the two methods we discussed earlier:

1.  **Simplifying by combining fractions** (which doesn't involve multiplying by the LCM).
2.  **Clearing fractions** by multiplying *all* terms (including the LHS) by the LCM.

Here is the correct way to execute the simplification step you attempted:

***

## Correction of the Intermediate Step

When you reach the equation $\frac{w}{-2} = \frac{2}{3} - \frac{1}{6}$, you have two standard, correct ways to proceed to simplify the Right-Hand Side (RHS).

### Option A: Standard Simplification (Combining Fractions)


$$\frac{w}{-2} = \frac{2}{3} - \frac{1}{6}$$

1.  **Find common denominator for RHS:** (LCM is 6).
    $$\frac{w}{-2} = \frac{2 \cdot 2}{3 \cdot 2} - \frac{1}{6}$$

2.  **Combine:** (Not clearing denominator)
    $$\frac{w}{-2} = \frac{4}{6} - \frac{1}{6}$$   $$\frac{w}{-2} = \frac{3}{6}$$

3.  **Reduce:** (Here we are clearing the denominator)
    $$\frac{w}{-2} = \frac{1}{2}$$
    $$w = \frac{1}{2} \times \frac{-2}{1} = -1$$


This method moving the alike factors,

---

### Option B: Clearing Fractions (The Intent Behind Your Mistake)

$$\frac{w}{-2} = \frac{2}{3} - \frac{1}{6}$$

1.  **Multiply *all terms* by the LCM (6):**  

        why multiply all terms ? because we don't want fraction, to take the fractions we have to modify the equation, if we modify we have to do it on both side
    $$6 \cdot \left(\frac{w}{-2}\right) = 6 \cdot \left(\frac{2}{3}\right) - 6 \cdot \left(\frac{1}{6}\right)$$

2.  **Simplify (Cancel denominators):**
    $$(3)w = 2(2) - 1(1)$$   $$-3w = 4 - 1$$   $$-3w = 3$$

3.  **Solve for $w$:**
    $$w = \frac{3}{-3}$$   $$\mathbf{w = -1}$$

