# More 

## Multi way
**$$\mathbf{\frac{w}{-2} + \frac{1}{6} = \frac{2}{3}}$$**

*Method 1*
----

Remove $\frac{1}{6}$ by doing inverse $-\frac{1}{6}$ on both side

$$\frac{w}{-2} + \cancel{\frac{1}{6}} \cancel{-\frac{1}{6}} = \frac{2}{3} -\frac{1}{6}$$

Now remove $\frac{}{-2}$ by doind inverse $\times -2$

$$\frac{\cancel{-2} }{1}\times \frac{w}{\cancel{-2}}  = \frac{-2}{1} \times \frac{2}{3} -  \frac{-2}{1} \times \frac{1}{6}$$

in right side of the equation move  $\frac{-2}{1}$ out as common

$$w = \frac{-2}{1}(\frac{2}{3} - \frac{1}{6})$$

LCM (2, 3, 6) = 6

$$w = \frac{-2}{1}(\frac{2 \times 2}{3 \times 2} - \frac{1 \times 1}{6 \times 1}) =  \frac{-2}{1}(\frac{4}{6} - \frac{1}{6})$$

$$w = \frac{-2}{1}(\frac{\cancel{3}^1}{\cancel{6}^2}) = \frac{\cancel{-2}}{1} \times \frac{1}{\cancel{2}}$$

$$w = -1$$

*method 2*
---

Remove $\frac{1}{6}$ by doing inverse $-\frac{1}{6}$ on both side

$$\frac{w}{-2} + \cancel{\frac{1}{6}} \cancel{-\frac{1}{6}} = \frac{2}{3} -\frac{1}{6}$$

Convert the fraction to same unit LCM (3, 6)= 6

$$\frac{-w \times 3}{-2 \times 3} = \frac{2 \times 2}{3 \times 2} - \frac{1 \times 1}{6 \times 1}$$

$$\frac{-3w}{6} = \frac{4}{6} - \frac{1}{6}$$

Remove $\frac{}{6}$ by inverse 

$$\frac{\cancel{6}}{1} * \frac{-3w}{\cancel{6}} = (\frac{\cancel{6}}{1} * \frac{4}{\cancel{6}}) - ( \frac{\cancel{6}}{1} * \frac{1}{\cancel{6}})$$

$$-3w = 3$$

remove -3 from w, -3 is multiplied to w so we have to divide as per iversion

$$\frac{\cancel{-3}w}{\cancel{-3}} = \frac{\cancel{3}}{-\cancel{3}}$$

$$w = -1$$

*Method 3*
----

clear Fraction 1st

$$\frac{w}{-2} + \frac{1}{6} = \frac{2}{3}$$

LCM(2, 6, 3) = 6

$$\frac{3w}{-6} + \frac{1}{6} = \frac{4}{6}$$

clear $\frac{}{6} \text{ by } \times 6$ 

$$-3w + 1 = 4$$

clear $+1 \text{ by } -1$

$$-3w \cancel{+1}\cancel{-1} = 4 -1$$

$$-3w = 3$$

remove -3 from w, -3 is multiplied to w so we have to divide as per iversion

$$\frac{\cancel{-3}w}{\cancel{-3}} = \frac{\cancel{3}}{-\cancel{3}}$$

$$w = -1$$

*method 4*
----

1.  **Isolate the variable term** by subtracting $\frac{1}{6}$ from both sides:
    $$\frac{w}{-2} = \frac{2}{3} - \frac{1}{6}$$

2.  **Simplify the RHS** by finding a common denominator (LCM is 6):
    $$\frac{w}{-2} = \frac{2 \times 2}{3 \times 2} - \frac{1 \times 1}{6 \times 1}$$
    $$\frac{w}{-2} = \frac{4}{6} - \frac{1}{6}$$

> [!NOTE]  
> Here we have may have a doubt about balancing the equation on LHS also, ($\frac{3w}{-6}$ instead of $\frac{w}{-2}$ )
> Actually we are not balancing the equation in this step, because equation is already balanced, ($\frac{2}{3}, \frac{1}{6}$) both are in different form. So we are simplying the equation to get equation   
> Summary: By finding **LCM** we are not changing the equation, we are just simplfying. This is applicable to equations above and different equation


3.  **Combine the fractions on the RHS:**
    $$\frac{w}{-2} = \frac{3}{6}$$

4.  **Reduce the fraction on the RHS:**
    $$\frac{w}{-2} = \frac{1}{2}$$

5.  **Isolate $w$** by multiplying both sides by $-2$:
    $$(-2) \times \frac{w}{-2} = (-2) \times \frac{1}{2}$$
    $$w = -\frac{2}{2}$$
    $$\mathbf{w = -1}$$


*Method 5*
---

1.  **Multiply *all terms* by the LCM (6):**  

    $$6 \cdot \left(\frac{w}{-2}\right) = 6 \cdot \left(\frac{2}{3}\right) - 6 \cdot \left(\frac{1}{6}\right)$$

2.  **Simplify :**
    $$(3)w = 2(2) - 1(1)$$   $$-3w = 4 - 1$$   $$-3w = 3$$

3.  **Solve for $w$:**
    $$w = \frac{3}{-3}$$   $$\mathbf{w = -1}$$

> [!IMPORTANT]  
> read this: [refer](lcm.md)  

**Verify**

Substitue $ w = -1$
$$\frac{-1}{-2} + \frac{1}{6}$$
$$\frac{1}{2} + \frac{1}{6}$$

LCM(2, 6) = 6

$$\frac{1 \times 3}{2 \times 3} + \frac{1 \times 1}{6 \times 1}$$
$$\frac{3}{6} + \frac{1}{6}$$
$$\frac{4}{6} = \frac{2}{3}$$

$$\frac{2}{3}=\frac{2}{3} \text{ is proved}$$

***
---

## variable on both sides

$$3x + 7 = 5x - 1$$


## more alike term

$$9 - 4y + 11y = 2y - 1 + 15$$


## combination of int, float, decimal(0.1, 0.001), many single variable on both side

$$0.2z + 5 - z + 1.5 = 10 - 4z + 0.3$$
$$4.5k - 7 + 1.05k = 12.0005 - 2k + 0.5$$

$$
\frac{1}{3}x + 2.5 - 5 = \frac{5}{6}x + 1\frac{1}{2} - 0.75x
$$
$$
\frac{3}{4}w - 1.25 + 7 = 2.5w + \frac{1}{5} - 0.003w
$$

$$
5(2.5x - 3) + \frac{1}{2}x = 4.08 - \frac{3}{4}(x + 0.004)
$$

$$
\frac{2}{5}\left(x - 3.5\right) + 1.05 = 4 - 0.1\left(\frac{1}{4}x + 7\right)
$$
