## Practice
Problems is a system of two linear equations in two variables ($x$ and $y$). It is a single problem that requires you to find the unique ordered pair $(\mathbf{x, y})$ that satisfies both equtions simultaneously.


## Problem 1: Mixed Decimals and Simple Fractions


$$\begin{cases} 0.25x - 0.5(y + 3) = 1.5 \\ \frac{1}{3}(2x - 1) + \frac{5}{6}y = \frac{1}{2} \end{cases}$$

1. The first equation is:$$0.25x - 0.5(y + 3) = 1.5$$
Multiply by 4 to eliminate the decimals:
$$4 \times [0.25x - 0.5(y + 3)] = 4 \times 1.5$$
$$x - 2(y + 3) = 6$$
$$x - 2y - 6 = 6$$

$$x - 2y = 6 + 6$$
$$\mathbf{x - 2y = 12}$$

Solve for X
$$x = 12 + 2y $$

Solve for Y
$$-2y = 12 - x$$

$$y = \frac{12 - x}{-2}$$

$$y = \frac{12}{-2} - \frac{x}{-2}$$
$$\mathbf{y = -6 + \frac{1}{2}x}$$

If we substitute x and y in same equation we can verify the answer is that right or not

If we substitute x or y in other equation we will find the system of equation

**Verify**

$$x-2y=12$$

substitute x 

$$x = 12+2y$$

$$12+2y-2y = 12$$
$$12=12$$
X is verified

substitute y

$$x-2(-6+\frac{1}{2}x)=12$$
$$x+12-\frac{2}{2}x=12$$
$$x+12-x=12$$
$$12=12$$
Y is verified

2. The second equation is:$$\frac{1}{3}(2x - 1) + \frac{5}{6}y = \frac{1}{2}$$
Multiply by the least common multiple of the denominators (3, 6, and 2), which is 6:$$6 \times \left[\frac{1}{3}(2x - 1) + \frac{5}{6}y\right] = 6 \times \frac{1}{2}$$
$$2(2x - 1) + 5y = 3$$
$$4x - 2 + 5y = 3$$
$$4x + 5y = 3 + 2$$
$$\mathbf{4x + 5y = 5}$$

Solve for x
$$4x = 5 - 5y$$
$$x = \frac{5 -5y}{4}$$

Solve for y
$$5y=5-4x$$
$$y=\frac{5-4x}{5}$$

$$y=1-\frac{4x}{5}$$

**Verify**

$$4x+5y=5$$

Substitute x
$$4(\frac{5-5y}{4})+5y=5$$

$$5-5y+5y=5$$

$$5=5$$
X is verified

Substitute y
$$4x+5(1 - \frac{4x}{5})=5$$

$$4x+5 - 5 \cdot\frac{4x}{5} = 5$$

$$4x+5-4x=5$$
$$5=5$$

### Substitution Method

**Now find the system of equation**

To Find system of equation substitute x or y from the equation 1 to the equation 2
If you substitute eq1 x to eq2, you will get y ponit and substitute that y to get x point

Equation 1  
$$0.25x - 0.5(y + 3) = 1.5 == x-2y=12$$
$$\begin{cases} x = 12+2y \\ y = -6 + \frac{1}{2}x \end{cases}$$

Equation 2
$$\frac{1}{3}(2x - 1) + \frac{5}{6}y = \frac{1}{2} == 4x+5y=5$$
$$\begin{cases} x = \frac{5 - 5y}{4} \\ y = 1-\frac{4x}{5} \end{cases}$$

#### Solve for y

**Sub x of eq 1 in eq 2**

$$\frac{1}{3}(2(12+2y) - 1) + \frac{5}{6}y = \frac{1}{2}$$
$$\frac{1}{3}((24+4y) - 1) + \frac{5}{6}y = \frac{1}{2}$$

LCM of 3, 6 and 2 is 6

$$6 \cdot \frac{1}{3}((24+4y) - 1) + 6 \cdot \frac{5}{6}y = 6 \cdot \frac{1}{2}$$

$$2\cdot(24+4y-1) +5y=3$$

$$48+8y-2 + 5y = 3$$

$$46+13y=3$$

$$13y=3-46$$
$$13y=-43$$
$$y=\frac{-43}{13}$$


**Sub x of eq 2 in eq 1**

Separate the fraction term:
$$\frac{5}{4} - \frac{5y}{4} - 2y = 12$$

Isolate the $y$ terms on the left and move the constant term ($\frac{5}{4}$) to the right:
$$-\frac{5y}{4} - 2y = 12 - \frac{5}{4}$$

Combine the $y$ terms on the left:

To combine $-\frac{5y}{4}$ and $-2y$, find a common denominator, which is 4.
$$-2y = -\frac{2y \times 4}{4} = -\frac{8y}{4}$$
So, the left side becomes:
$$-\frac{5y}{4} - \frac{8y}{4} = \frac{-5y - 8y}{4} = -\frac{13y}{4}$$

Combine the constant terms on the right:

To combine $12$ and $-\frac{5}{4}$, find a common denominator, which is 4.
$$12 = \frac{12 \times 4}{4} = \frac{48}{4}$$
So, the right side becomes:
$$\frac{48}{4} - \frac{5}{4} = \frac{48 - 5}{4} = \frac{43}{4}$$

Equate the simplified sides:
$$-\frac{13y}{4} = \frac{43}{4}$$

Solve for $y$:
Since the denominators on both sides are the same (4), the numerators must be equal:
$$-13y = 43$$

Divide by $-13$:
$$y = \frac{43}{-13}$$
$$\mathbf{y = -\frac{43}{13}}$$

The result is the same, confirming the previous solution.

#### Solve for x

**Sub y of eq 1 in eq 2**

$$\begin{align*} 
4x + 5\left(-6 + \frac{1}{2}x\right) &= 5 \\
4x - 30 + \frac{5}{2}x &= 5 \\
4x + \frac{5}{2}x &= 5 + 30 \\
\frac{8}{2}x + \frac{5}{2}x &= 35 \\
\frac{13}{2}x &= 35 \\
x &= 35 \cdot \frac{2}{13} \\
\mathbf{x} &= \mathbf{\frac{70}{13}} 
\end{align*}$$

**Sub y of eq 2 in eq 1**
$$x - 2\left(1-\frac{4x}{5}\right) = 12$$
$$x - 2 + \frac{8x}{5} = 12$$
$$x + \frac{8x}{5} = 14$$
$$\frac{5x}{5} + \frac{8x}{5} = 14$$
$$\frac{5x + 8x}{5} = 14$$
$$\frac{13x}{5} = 14$$
$$13x = 14 \times 5$$
$$13x = 70$$
$$x = \frac{70}{13}$$

The result is the same, confirming the previous solution.

#### Solve for other variable

**Substitute $y = -\frac{43}{13}$ into the equation 2:**
$$\frac{1}{3}(2x - 1) + \frac{5}{6}\left(-\frac{43}{13}\right) = \frac{1}{2}$$

$$\frac{1}{3}(2x - 1) - \frac{5 \times 43}{6 \times 13} = \frac{1}{2}$$

Simplify the constant term:
$$\frac{1}{3}(2x - 1) - \frac{215}{78} = \frac{1}{2}$$


Multiply the entire equation by the least common multiple (LCM) of the denominators (3, 78, and 2), which is **78**:

$$78 \times \left[ \frac{1}{3}(2x - 1) - \frac{215}{78} \right] = 78 \times \frac{1}{2}$$

$$26(2x - 1) - 215 = 39$$

Distribute the $26$:
$$52x - 26 - 215 = 39$$

Combine the constant terms on the left:
$$52x - 241 = 39$$

Add $241$ to both sides:
$$52x = 39 + 241$$
$$52x = 280$$

Divide by $52$:
$$x = \frac{280}{52}$$

Divide both the numerator and the denominator by their greatest common divisor, which is 4:
$$x = \frac{280 \div 4}{52 \div 4}$$
$$\mathbf{x = \frac{70}{13}}$$

This result was confirmed by the calculation:
$x = \frac{70}{13}$

**substitute $y = -\frac{43}{13}$ into the equation 1:**

The first equation is:
$$0.25x - 0.5(y + 3) = 1.5$$

Substitute $\mathbf{y = -\frac{43}{13}}$ into the equation:
$$0.25x - 0.5\left(-\frac{43}{13} + 3\right) = 1.5$$

Simplify the Term in Parentheses

First, find a common denominator for the terms inside the parentheses:
$$-\frac{43}{13} + 3 = -\frac{43}{13} + \frac{3 \times 13}{13} = -\frac{43}{13} + \frac{39}{13} = \frac{-43 + 39}{13} = \mathbf{-\frac{4}{13}}$$

Now, substitute this result back into the equation:
$$0.25x - 0.5\left(-\frac{4}{13}\right) = 1.5$$


Multiply the decimal values (or their fraction equivalents, $\frac{1}{2}$ and $\frac{1}{4}$):
$$0.5 \times \left(-\frac{4}{13}\right) = \frac{1}{2} \times \left(-\frac{4}{13}\right) = -\frac{4}{26} = -\frac{2}{13}$$

The equation is now:
$$0.25x - \left(-\frac{2}{13}\right) = 1.5$$

* $$0.25=\frac{1}{4}, 1.5 = \frac{3}{2}$$
$$\frac{1}{4}x + \frac{2}{13} = \frac{3}{2}$$

Subtract $\frac{2}{13}$ from both sides:
$$\frac{1}{4}x = \frac{3}{2} - \frac{2}{13}$$

Find a common denominator for the right side (LCM of 2 and 13 is 26):
$$\frac{1}{4}x = \frac{3 \times 13}{2 \times 13} - \frac{2 \times 2}{13 \times 2}$$
$$\frac{1}{4}x = \frac{39}{26} - \frac{4}{26}$$
$$\frac{1}{4}x = \frac{35}{26}$$

Multiply both sides by $4$:
$$x = 4 \times \frac{35}{26}$$
$$x = \frac{140}{26}$$

Simplify the fraction by dividing the numerator and denominator by their greatest common divisor, 2:
$$x = \frac{140 \div 2}{26 \div 2}$$
$$\mathbf{x = \frac{70}{13}}$$

The result confirms the solution for $x$.

**Substitute $x = \frac{70}{13}$ into the equation 1**

$x = \frac{70}{13}$ into Equation 1: $y = 1 - \frac{4x}{5}$

$$y = 1 - \frac{4}{5} \left(\frac{70}{13}\right)$$

First, simplify the multiplication:
$$y = 1 - \frac{4 \times 70}{5 \times 13}$$
$$y = 1 - \frac{280}{65}$$

Simplify the fraction $\frac{280}{65}$ by dividing the numerator and denominator by $5$:
$$\frac{280 \div 5}{65 \div 5} = \frac{56}{13}$$

$$y = 1 - \frac{56}{13}$$

Express $1$ as $\frac{13}{13}$ to find a common denominator:
$$y = \frac{13}{13} - \frac{56}{13}$$
$$y = \frac{13 - 56}{13}$$
$$y = -\frac{43}{13}$$

**Substitute $x = \frac{70}{13}$ into the equation 2**

$x = \frac{70}{13}$ into Equation 2: $x - 2y = 12$

$$\frac{70}{13} - 2y = 12$$

Isolate the term with $y$ by subtracting $\frac{70}{13}$ from both sides:
$$-2y = 12 - \frac{70}{13}$$

Express $12$ as a fraction with a denominator of $13$: $12 = \frac{12 \times 13}{13} = \frac{156}{13}$.
$$-2y = \frac{156}{13} - \frac{70}{13}$$
$$-2y = \frac{156 - 70}{13}$$
$$-2y = \frac{86}{13}$$

Divide both sides by $-2$:
$$y = \frac{86}{13} \div (-2)$$
$$y = \frac{86}{13} \times \left(-\frac{1}{2}\right)$$

$$y = -\frac{86}{2 \times 13}$$
$$y = -\frac{43}{13}$$

####  Verification

Check the solution $(\mathbf{x, y}) = \left(\frac{70}{13}, -\frac{43}{13}\right)$ in the original simplified equations.

**In Equation 1 ($x - 2y = 12$):**
$$\frac{70}{13} - 2\left(-\frac{43}{13}\right) = \frac{70}{13} + \frac{86}{13} = \frac{70 + 86}{13} = \frac{156}{13} = 12$$
(Correct: $12 = 12$)

**In Equation 2 ($4x + 5y = 5$):**
$$4\left(\frac{70}{13}\right) + 5\left(-\frac{43}{13}\right) = \frac{280}{13} - \frac{215}{13} = \frac{280 - 215}{13} = \frac{65}{13} = 5$$
(Correct: $5 = 5$)

### Elimination Method

#### Eliminate $x$

To eliminate $x$, we need the coefficients of $x$ in both equations to be opposites (or the same, if we plan to subtract). The coefficient in Eq 1 is $1$, and in Eq 2 is $4$. We can multiply Equation 1 by $-4$.

$$\begin{cases} -4(x - 2y) = -4(12) \\ 4x + 5y = 5 \end{cases}$$

This gives us the modified system:
$$\begin{cases} -4x + 8y = -48 \quad \text{(Modified Eq 1)} \\ 4x + 5y = 5 \quad \text{(Equation 2)} \end{cases}$$

Add (Modified Eq 1) and (Equation 2) together:

$$(-4x + 8y) + (4x + 5y) = -48 + 5$$
$$-4x + 4x + 8y + 5y = -43$$
$$0x + 13y = -43$$
$$13y = -43$$
$$\mathbf{y = -\frac{43}{13}}$$

Substitute in any one of the equation to get x

#### Eliminate $y$

$$\begin{cases} x - 2y = 12 \quad \text{(Equation 1)} \\ 4x + 5y = 5 \quad \text{(Equation 2)} \end{cases}$$

The coefficients for $y$ are $-2$ and $5$. The least common multiple (LCM) of $2$ and $5$ is $10$. We want the $y$ terms to be $-10y$ and $+10y$.

1.  **Multiply Equation 1 by 5** to get $-10y$:
    $$5 \times (x - 2y) = 5 \times 12$$
    $$5x - 10y = 60 \quad \text{(Modified Eq 1)}$$

2.  **Multiply Equation 2 by 2** to get $+10y$:
    $$2 \times (4x + 5y) = 2 \times 5$$
    $$8x + 10y = 10 \quad \text{(Modified Eq 2)}$$

The new system is:
$$\begin{cases} 5x - 10y = 60 \\ 8x + 10y = 10 \end{cases}$$

Now, **add** the two modified equations together:

$$\begin{array}{rcl} 5x - 10y &= &60 \\ + \quad 8x + 10y &= &10 \\ \hline 13x + 0y &= &70 \end{array}$$

The $y$ terms have been eliminated, leaving an equation with only $x$:
$$13x = 70$$

Divide both sides by $13$:
$$\mathbf{x = \frac{70}{13}}$$

## Problem 2: Nested Fractions and Decimals

This system involves complex nested fractions that must be simplified first before clearing the denominators.

$$\begin{cases} \frac{x}{0.1} - \frac{y}{0.05} = 40 \\ \frac{1}{2}\left( \frac{x}{4} + \frac{y}{5} \right) = \frac{1}{10} \end{cases}$$

* **Hint:** Simplify $\frac{x}{0.1} = 10x$ and $\frac{y}{0.05} = 20y$ in Equation 1. For Equation 2, clear the outer fraction first by multiplying by 2, then clear the inner fractions.

---

### Problem 3: Distributive Property with Complex Coefficients

This system requires heavy use of the distributive property with fractional and decimal coefficients.

$$\begin{cases} 0.5(x - 2y) - 0.75x = \frac{3}{4}y + 1 \\ \frac{2}{3}x - \frac{1}{6}(y + 4) = \frac{1}{2}(x - y) \end{cases}$$

* **Hint:** Convert all decimals to fractions (e.g., $0.5 = 1/2$, $0.75 = 3/4$). Simplify each side of both equations separately before attempting to clear the denominators.

---

### Problem 4: System with Reciprocal Variables (Requires Substitution)

While technically not a linear equation in $x$ and $y$, this common type of problem can be *transformed* into a linear system using substitution, which is a crucial advanced technique.

$$\begin{cases} \frac{2}{x} + \frac{3}{y} = 12 \\ \frac{1}{x} - \frac{4}{y} = -5 \end{cases}$$

* **Hint:** Let $\mathbf{u = \frac{1}{x}}$ and $\mathbf{v = \frac{1}{y}}$. Solve the resulting linear system for $u$ and $v$ first, then use those values to find $x$ and $y$.

---

### Problem 5: Absolute Value Coefficients (Conceptual Challenge)

This problem tests your understanding of the relationship between coefficients, leading to a special case (No Solution or Infinitely Many Solutions).

$$\begin{cases} \frac{1}{4}x - 0.3y = 2 \\ \frac{5}{8}x - 0.6y = 3 \end{cases}$$

* **Hint:** Convert $0.3 = 3/10$ and $0.6 = 6/10 = 3/5$. Clear the fractions in both equations. If you solve by elimination, you will find a contradiction. **Pay attention to the relationship between the final $x$ and $y$ coefficients and the constants.**




## Solutions to the Challenging Systems of Linear Equations

| Problem | Simplified System (Standard Form) | Final Solution ($\mathbf{x, y}$) |
| :---: | :---: | :---: |
| **Problem 1** | $\begin{cases} x - 2y = 12 \\ 4x + 5y = 5 \end{cases}$ | $\mathbf{(x, y) = (5, -3)}$ |
| **Problem 2** | $\begin{cases} 10x - 20y = 40 \\ x/4 + y/5 = 1/5 \implies 5x + 4y = 4 \end{cases}$ | $\mathbf{(x, y) = (2, -1)}$ |
| **Problem 3** | $\begin{cases} -x - 5y = 4 \\ x - y = 4 \end{cases}$ | $\mathbf{(x, y) = (1, -3)}$ |
| **Problem 4** | $\begin{cases} 2u + 3v = 12 \\ u - 4v = -5 \end{cases}$ | $\mathbf{(x, y) = (1/3, 1/2)}$ |
| **Problem 5** | $\begin{cases} 5x - 12y = 40 \\ 5x - 12y = 24 \end{cases}$ | **No Solution** |

***

### Notes on Special Cases

* **Problem 4: Reciprocal Variables**
    * The linear substitution system is $2u + 3v = 12$ and $u - 4v = -5$.
    * The solution to the $u, v$ system is $\mathbf{(u, v) = (3, 2)}$.
    * Since $x = 1/u$ and $y = 1/v$, the final solution is $\mathbf{(x, y) = (1/3, 1/2)}$.

* **Problem 5: No Solution (Inconsistent System)**
    * After clearing the fractions and decimals, the simplified system becomes:
        $$\begin{cases} 5x - 12y = 40 \\ 5x - 12y = 24 \end{cases}$$
    * When you attempt to eliminate $x$ and $y$ (by subtracting the second equation from the first), you get the false statement $\mathbf{0 = 16}$.
    * This means the two equations represent **parallel lines** that never intersect, so there is **No Solution**.

# Inequalties

$$\begin{cases} y > 2x - 1  \\ y \le -x + 4 & \end{cases}$$

Find the Intersection Point

$$2x - 1 = -x + 4$$
$$2x + x = 4 + 1$$
$$3x = 5$$
$$x = \frac{5}{3}$$

Now, substitute $x = \frac{5}{3}$  into either equation (using $y = -x + 4$):
$$y = -\left(\frac{5}{3}\right) + 4$$

$$y = -\frac{5}{3} + \frac{12}{3}$$

$$y = \frac{7}{3}$$

The intersection point is $\left(\frac{5}{3}, \frac{7}{3}\right)$, which is approximately $(1.67, 2.33)$. This point is not included in the solution because the first inequality is strict ($>$).